

Problem Set3

Kaiqu Liang; Zirun Hong; Jitian Zheng

March 14, 2018

Question1

(a)

Proof: I will prove $\forall n \in \mathbb{N}, F_n - 2 = \prod_{i=0}^{n-1} F_i$ by induction on n

Base case: $n = 0$

Left hand side: $F_0 - 2 = 2^{2^0} + 1 - 2 = 2^1 + 1 - 2 = 1$

Right hand side: Since $0 > -1$, $\prod_{i=0}^{-1} F_i = 1$

Therefore we have $F_0 - 2 = \prod_{i=0}^{-1} F_i$

Hence $F_n - 2 = \prod_{i=0}^{n-1} F_i$ is True for $n = 0$

Inductive step: Let $k \in \mathbb{N}$. Assume $F_k - 2 = \prod_{i=0}^{k-1} F_i$

WTS: $F_{k+1} - 2 = \prod_{i=0}^k F_i$

Since we know $F_k = 2^{2^k} + 1$

$F_{k+1} - 2 = 2^{2^{k+1}} + 1 - 2 = 2^{2^{k+1}} - 1$

$$\begin{aligned} \prod_{i=0}^k F_i &= \prod_{i=0}^{k-1} F_i * F_k \\ &= (F_k - 2) * F_k && \text{(by induction hypothesis)} \\ &= (2^{2^k} + 1 - 2)(2^{2^k} + 1) && \text{(by definition of } F_k) \\ &= (2^{2^k} - 1)(2^{2^k} + 1) \\ &= (2^{2^k})^2 - 1 \\ &= 2^{2^{k+1}} - 1 \end{aligned}$$

Therefore we have $F_{k+1} - 2 = \prod_{i=0}^k F_i$

By base case and inductive step, I can conclude that $\forall n \in \mathbb{N}, F_n - 2 = \prod_{i=0}^{n-1} F_i$

Question2

(a)

$$a_0 = 1$$

$$a_1 = \frac{1}{\frac{1}{a_0} + 1} = \frac{1}{1+1} = \frac{1}{2}$$

$$a_2 = \frac{1}{\frac{1}{a_1} + 1} = \frac{1}{\frac{1}{\frac{1}{2}} + 1} = \frac{1}{3}$$

$$a_3 = \frac{1}{\frac{1}{a_2} + 1} = \frac{1}{\frac{1}{\frac{1}{3}} + 1} = \frac{1}{4}$$

(b)

$$\forall n \in \mathbb{N}, a_n = \frac{1}{n+1}$$

Proof: I will prove $\forall n \in \mathbb{N}, a_n = \frac{1}{n+1}$ by induction on n

Base case: $n = 0$

Left hand side: We know $a_0 = 1$

Right hand side: $\frac{1}{n+1} = \frac{1}{0+1} = 1$

Therefore $a_n = \frac{1}{n+1}$ is true when $n = 0$

inductive step: Let $k \in \mathbb{N}$. Assume $a_k = \frac{1}{k+1}$

WTS: $a_{k+1} = \frac{1}{k+2}$

We will calculate starting from the left side and show that it equals the right side

$$\begin{aligned} a_{k+1} &= \frac{1}{\frac{1}{a_k} + 1} && \text{(by definition of } a_{k+1}) \\ &= \frac{1}{\frac{1}{\frac{1}{k+1}} + 1} && \text{(by induction hypothesis)} \\ &= \frac{1}{k+1+1} \\ &= \frac{1}{k+2} \end{aligned}$$

I have shown that $a_{k+1} = \frac{1}{k+2}$

By base case and inductive step, I can conclude that $\forall n \in \mathbb{N}, a_n = \frac{1}{n+1}$

(c)

Since we know $\forall k \in \mathbb{N}, k > 1 \Rightarrow a_{k,0} = k$

We have $a_{2,0} = 2$

Since $\forall n \in \mathbb{N}, a_{k,n+1} = \frac{k}{\frac{1}{a_{k,n}} + 1}$

$$a_{2,1} = \frac{2}{\frac{1}{a_{2,0}} + 1} = \frac{2}{\frac{1}{2} + 1} = \frac{2}{\frac{3}{2}} = 2 \times \frac{2}{3} = \frac{4}{3}$$

$$a_{2,2} = \frac{2}{\frac{1}{a_{2,1}} + 1} = \frac{2}{\frac{1}{\frac{4}{3}} + 1} = \frac{2}{\frac{3}{4} + 1} = \frac{8}{7}$$

$$a_{2,3} = \frac{2}{\frac{1}{a_{2,2}} + 1} = \frac{2}{\frac{1}{\frac{8}{7}} + 1} = \frac{2}{\frac{7}{8} + 1} = \frac{16}{15}$$

Similarly, $a_{3,0} = 3$

$$a_{3,1} = \frac{3}{\frac{1}{a_{3,0}} + 1} = \frac{3}{\frac{1}{3} + 1} = \frac{9}{4}$$

$$a_{3,2} = \frac{3}{\frac{1}{a_{3,1}} + 1} = \frac{3}{\frac{1}{\frac{9}{4}} + 1} = \frac{27}{13}$$

$$a_{3,3} = \frac{3}{\frac{1}{a_{3,2}} + 1} = \frac{3}{\frac{13}{27} + 1} = \frac{81}{40}$$

(d)

I want to prove: $\forall k \in \mathbb{N}, \forall n \in \mathbb{N}, k > 1 \Rightarrow a_{k,n} = \frac{k^{n+2} - k^{n+1}}{k^{n+1} - 1}$

proof: Let $k \in \mathbb{N}$

I will prove $\forall n \in \mathbb{N}, k > 1 \Rightarrow a_{k,n} = \frac{k^{n+2} - k^{n+1}}{k^{n+1} - 1}$ by induction on n .

Base case: $n = 0$. Assume $k > 1$

Left hand side: $a_{k,0} = k$ (by definition of $a_{k,0}$)

Right hand side: $\frac{k^{n+2} - k^{n+1}}{k^{n+1} - 1} = \frac{k^2 - k}{k - 1} = \frac{k(k-1)}{k-1} = k$

Therefore we have $a_{k,n} = \frac{k^{n+2} - k^{n+1}}{k^{n+1} - 1}$ is true when $n = 0$

Inductive step: Let $n \in \mathbb{N}$ Assume $a_{k,n} = \frac{k^{n+2} - k^{n+1}}{k^{n+1} - 1}, k > 1$

WTS: $a_{k,n+1} = \frac{k^{n+3} - k^{n+2}}{k^{n+2} - 1}$

We will start from the left side and show that it equals the right side.

$$\begin{aligned} a_{k,n+1} &= \frac{k}{\frac{1}{a_{k,n}} + 1} && \text{(by definition of } a_{k,n+1}) \\ &= \frac{k}{\frac{1}{\frac{k^{n+2} - k^{n+1}}{k^{n+1} - 1}} + 1} && \text{(by induction hypothesis)} \\ &= \frac{k}{\frac{k^{n+1} - 1}{k^{n+2} - k^{n+1}} + 1} \\ &= \frac{k(k^{n+2} - k^{n+1})}{k^{n+1} - 1 + k^{n+2} - k^{n+1}} \\ &= \frac{k^{n+3} - k^{n+2}}{k^{n+2} - 1} \end{aligned}$$

I have shown that $a_{k,n+1} = \frac{k^{n+3} - k^{n+2}}{k^{n+2} - 1}$

By base case and inductive step, I can conclude that $\forall n \in \mathbb{N}, k > 1 \Rightarrow a_{k,n} = \frac{k^{n+2} - k^{n+1}}{k^{n+1} - 1}$

Therefore $\forall k \in \mathbb{N}, \forall n \in \mathbb{N}, k > 1 \Rightarrow a_{k,n} = \frac{k^{n+2} - k^{n+1}}{k^{n+1} - 1}$

Question3

(a)

Let $f: \mathbb{N} \rightarrow \mathbb{R}^{\geq 0}$

Assume $f \in \mathcal{O}(n^2)$. By definition of big-Oh, $\exists c_1, n_1 \in \mathbb{R}^+, \forall n \in \mathbb{N}, n \geq n_1 \Rightarrow f(n) \leq c_1 \cdot n$

WTS: $\text{Sum}_f \in \mathcal{O}(n^2)$ which is equivalent to show $\exists c, n_0 \in \mathbb{R}^+, \forall n \in \mathbb{N}, n \geq n_0 \Rightarrow \sum_{i=0}^n f(i) \leq cn^2$

Let $c = c_1 + \sum_{i=0}^{n_1} f(i)$

Let $n_0 = n_1$

Let $n \in \mathbb{N}$

Assume $n \geq n_0$. Hence $n \geq n_1$,

Therefore we have $f(n) \leq c_1 \cdot n$

$$\begin{aligned}
\text{Then } \sum_{i=0}^n f(i) &= \sum_{i=0}^{n_1} f(i) + \sum_{i=n_1+1}^n f(i) && \text{(break up summations)} \\
&= \sum_{i=0}^{n_1} f(i) + f(n_1+1) + f(n_1+2) + \dots + f(n) \\
&\leq \sum_{i=0}^{n_1} f(i) + c_1 \frac{(n_1+1+n)(n-n_1)}{2} \\
&= \sum_{i=0}^{n_1} f(i) + \frac{c_1}{2}(n^2 + n - n_1^2 - n_1) \\
&= \sum_{i=0}^{n_1} f(i) + \frac{c_1}{2}n^2 + \frac{c_1}{2}n - \frac{c_1}{2}(n_1^2 + n_1)
\end{aligned}$$

Since $c_1 > 0, n_1 > 0, -\frac{c_1}{2}(n_1^2 + n_1) < 0$

Since $c_1 > 0, n_1 > 0, n \geq n_0$

We get $n > 0$, therefore $n \geq 1$

Hence $\frac{c_1}{2}n(n-1) \geq 0$

$\frac{c_1}{2}n \leq \frac{c_1}{2}n^2$

Since $\text{Sum}_f(n_1) \geq 0, n^2 - 1 \geq 0$

We have $\sum_{i=0}^{n_1} f(i) \cdot (n^2 - 1) \geq 0$

Therefore $\sum_{i=0}^{n_1} f(i) \leq \sum_{i=0}^{n_1} f(i) \cdot n^2$

Hence $\sum_{i=0}^{n_1} f(i) + \frac{c_1}{2}n^2 + \frac{c_1}{2}n - \frac{c_1}{2}(n_1^2 + n_1)$

$\leq \frac{c_1}{2}n^2 + \frac{c_1}{2}n^2 + \sum_{i=0}^{n_1} f(i) \cdot n^2$

$= (c_1 + \sum_{i=0}^{n_1} f(i)) \cdot n^2$

$= cn^2$

I have shown that $\sum_{i=0}^n f(i) \leq cn^2$

I can conclude that $\forall f : \mathbb{N} \rightarrow \mathbb{R}^{\geq 0}$, if $f \in \mathcal{O}(n)$, then $\text{Sum}_f \in \mathcal{O}(n^2)$

(b)

I will prove $\forall n \in \mathbb{N}, \sum_{i=1}^{2^n} \frac{1}{i} \geq \frac{n}{2}$ by induction on n

Base case: $n = 0$

Left hand side: $\sum_{i=1}^{2^0} \frac{1}{i} = \sum_{i=1}^{2^0} \frac{1}{i} = 1$

Right hand side: $\frac{n}{2} = \frac{0}{2} = 0$

Therefore $\sum_{i=1}^{2^n} \frac{1}{i} \geq \frac{n}{2}$ is true when $n = 0$

Inductive step: Let $k \in \mathbb{N}$. Assume $\sum_{i=1}^{2^k} \frac{1}{i} \geq \frac{k}{2}$

WTS: $\sum_{i=1}^{2^{k+1}} \frac{1}{i} \geq \frac{k+1}{2}$

I will calculate starting from the left side and show that it is greater or equal than the right hand side.

$$\begin{aligned}
\sum_{i=1}^{2^{k+1}} \frac{1}{i} &= \sum_{i=1}^{2^k} \frac{1}{i} + \sum_{i=2^k+1}^{2^{k+1}} \frac{1}{i} && \text{(break up summations)} \\
&\geq \frac{k}{2} + \sum_{i=2^k+1}^{2^{k+1}} \frac{1}{i} && \text{(by induction hypothesis)} \\
&= \frac{k}{2} + \frac{1}{2^k+1} + \frac{1}{2^k+2} + \dots + \frac{1}{2^k+2^k} \\
&\geq \frac{k}{2} + \frac{1}{2^k+2^k} + \frac{1}{2^k+2^k} + \dots + \frac{1}{2^k+2^k} \\
&= \frac{k}{2} + \frac{2^k}{2^{k+1}} \\
&= \frac{k+1}{2}
\end{aligned}$$

I have shown that $\sum_{i=1}^{2^{k+1}} \frac{1}{i} \geq \frac{k+1}{2}$

Therefore I can conclude that $\forall n \in \mathbb{N}, \sum_{i=1}^{2^n} \frac{1}{i} \geq \frac{n}{2}$

(c)

Disprove: $\forall f, g : \mathbb{N} \rightarrow \mathbb{R}^{\geq 0}, f(n) \in \mathcal{O}(g(n)) \Rightarrow \text{Sum}_f(n) \in \mathcal{O}(n \cdot g(n))$ which is equivalent to $\forall f, g : \mathbb{N} \rightarrow \mathbb{R}^{\geq 0}, [\exists c_1, n_1 \in \mathbb{R}^+, \forall n \in \mathbb{N}, n \geq n_1 \Rightarrow f(n) \leq c_1 g(n)] \Rightarrow [\exists c, n_0 \in \mathbb{R}^+, \forall n \in \mathbb{N}, n \geq n_0 \Rightarrow \sum_{i=0}^n f(i) \leq c \cdot n \cdot g(n)]$

To disprove the statement, I want to prove the negation.

The negation: $\exists f, g : \mathbb{N} \rightarrow \mathbb{R}^{\geq 0}, [\exists c_1, n_1 \in \mathbb{R}^+, \forall n \in \mathbb{N}, n \geq n_1 \Rightarrow f(n) \leq c_1 g(n)] \wedge [\forall c, n_0 \in \mathbb{N}, \exists n \in \mathbb{N}, n \geq n_0 \wedge \sum_{i=0}^n f(i) > c \cdot n \cdot g(n)]$

Let $f(n) = \frac{1}{n+1}$, Let $g(n) = \frac{1}{2n}$

First I want to show: $\exists c_1, n_1 \in \mathbb{R}^+, \forall n \in \mathbb{N}, n \geq n_1 \Rightarrow f(n) \leq c_1 \cdot g(n) (*)$

Let $c_1 = 2, n_1 = 1$. Let $n \in \mathbb{N}$

Assume $n \geq n_1$, therefore $n \geq 1$

Since $n+1 \geq n > 0$

We have $\frac{1}{n+1} \leq \frac{1}{n}$

Then $\frac{1}{n+1} \leq \frac{1}{2n} \times 2$

$f(n) \leq c_1 \cdot g(n)$

I have shown that $\exists c_1, n_1 \in \mathbb{R}^+, \forall n \in \mathbb{N}, n \geq n_1 \Rightarrow f(n) \leq c_1 g(n)$

Second I want to show: $\forall c, n_0 \in \mathbb{N}, \exists n \in \mathbb{N}, n \geq n_0 \wedge [\sum_{i=0}^n f(i) > c \cdot n \cdot g(n)] (*)$

Let $c, n_0 \in \mathbb{R}^+$

Let $n = \lceil n_0 \rceil + 2^{\lceil c \rceil}$

By definition of ceiling function, we have $2^{\lceil c \rceil} \geq 2^c \geq 0$

$\lceil n_0 \rceil \geq n_0$

Therefore $2^{\lceil c \rceil} + \lceil n_0 \rceil \geq n_0$

We get $n \geq n_0$

Next, WTS: $\sum_{i=0}^n f(i) > c \cdot n \cdot g(n)$

I will start from the left side:

$\sum_{i=0}^n f(i) = \sum_{i=0}^{\lceil n_0 \rceil + 2^{\lceil c \rceil}} \frac{1}{i+1}$

$$= \sum_{i=0}^{2^{\lceil c \rceil}-1} \frac{1}{i+1} + \sum_{i=2^{\lceil c \rceil}}^{\lceil n_0 \rceil + 2^{\lceil c \rceil}} \frac{1}{i+1} \text{ (break up summations)}$$

By conclusion of Question 3(b),

$$\text{We know } \sum_{i=1}^{2^{\lceil c \rceil}} \frac{1}{i} \geq \frac{\lceil c \rceil}{2}$$

$$\text{Since } \sum_{i=0}^{2^{\lceil c \rceil}-1} \frac{1}{i+1} = \sum_{i=1}^{2^{\lceil c \rceil}} \frac{1}{i}$$

$$\text{We also have } \sum_{i=0}^{2^{\lceil c \rceil}-1} \frac{1}{i+1} \geq \frac{\lceil c \rceil}{2}$$

Therefore

$$\begin{aligned} & \sum_{i=0}^{2^{\lceil c \rceil}-1} \frac{1}{i+1} + \sum_{i=2^{\lceil c \rceil}}^{\lceil n_0 \rceil + 2^{\lceil c \rceil}} \frac{1}{i+1} \\ & \geq \frac{\lceil c \rceil}{2} + \frac{1}{2^{\lceil c \rceil} + 1} + \frac{1}{2^{\lceil c \rceil} + 2} + \dots + \frac{1}{2^{\lceil c \rceil} + \lceil n_0 \rceil + 1} \\ & \geq \frac{\lceil c \rceil}{2} + \frac{1}{2^{\lceil c \rceil} + \lceil n_0 \rceil + 1} + \frac{1}{2^{\lceil c \rceil} + \lceil n_0 \rceil + 1} + \dots + \frac{1}{2^{\lceil c \rceil} + \lceil n_0 \rceil + 1} \\ & = \frac{\lceil c \rceil}{2} + \frac{\lceil n_0 \rceil + 1}{2^{\lceil c \rceil} + \lceil n_0 \rceil + 1} \\ & > \frac{\lceil c \rceil}{2} \quad \left(\text{Since } \frac{\lceil n_0 \rceil + 1}{2^{\lceil c \rceil} + \lceil n_0 \rceil + 1} > 0 \right) \\ & \geq \frac{c}{2} \quad \left(\text{by definition of ceiling function} \right) \end{aligned}$$

Then let's look at the right hand side:

$$\begin{aligned} c \cdot n \cdot g(n) &= c \cdot (\lceil n_0 \rceil + 2^{\lceil c \rceil}) \cdot \frac{1}{2(\lceil n_0 \rceil + 2^{\lceil c \rceil})} \quad \left(\text{by what we take for } g(n) \right) \\ &= \frac{c}{2} \end{aligned}$$

Therefore I have shown that $\sum_{i=0}^n f(i) > c \cdot n \cdot g(n)$

By * and (*), I can conclude that the negation is true.

Therefore the original statement is False.